More adjustments and fixes to the program logic and proof automation needed for compatibility with ExportClight compiler

progs/test1.v
@@ -2,21 +2,21 @@ Require Import Clightdefs.
 
 Local Open Scope Z_scope.
 
-Definition _main : ident := 15%positive.
-Definition _h : ident := 7%positive.
+Definition _p : ident := 8%positive.
+Definition _struct_list : ident := 5%positive.
+Definition _v : ident := 12%positive.
+Definition _sumlist : ident := 10%positive.
 Definition ___builtin_annot_intval : ident := 3%positive.
+Definition ___builtin_memcpy_aligned : ident := 2%positive.
 Definition ___builtin_fabs : ident := 1%positive.
 Definition _r : ident := 14%positive.
-Definition _s : ident := 9%positive.
-Definition _three : ident := 4%positive.
-Definition _p : ident := 8%positive.
-Definition _reverse : ident := 13%positive.
 Definition _t : ident := 6%positive.
-Definition _v : ident := 12%positive.
 Definition _w : ident := 11%positive.
-Definition _struct_list : ident := 5%positive.
-Definition ___builtin_memcpy_aligned : ident := 2%positive.
-Definition _sumlist : ident := 10%positive.
+Definition _three : ident := 4%positive.
+Definition _h : ident := 7%positive.
+Definition _s : ident := 9%positive.
+Definition _reverse : ident := 13%positive.
+Definition _main : ident := 15%positive.
 
 Definition t_struct_list :=
    (Tstruct _struct_list
@@ -39,27 +39,23 @@ Definition f_sumlist := {|
   fn_temps := ((_s, tint) :: (_t, (tptr t_struct_list)) :: (_h, tint) :: nil);
   fn_body :=
 (Ssequence
-  (Sset _s (Ecast (Econst_int (Int.repr 0) tint) tint))
+  (Sset _s (Econst_int (Int.repr 0) tint))
   (Ssequence
-    (Sset _t (Ecast (Etempvar _p (tptr t_struct_list)) (tptr t_struct_list)))
+    (Sset _t (Etempvar _p (tptr t_struct_list)))
     (Ssequence
       (Swhile
         (Etempvar _t (tptr t_struct_list))
         (Ssequence
           (Sset _h
-            (Ecast
-              (Efield
-                (Ederef (Etempvar _t (tptr t_struct_list)) t_struct_list) _h
-                tint) tint))
+            (Efield (Ederef (Etempvar _t (tptr t_struct_list)) t_struct_list)
+              _h tint))
           (Ssequence
             (Sset _t
-              (Ecast
-                (Efield
-                  (Ederef (Etempvar _t (tptr t_struct_list)) t_struct_list)
-                  _t (tptr t_struct_list)) (tptr t_struct_list)))
+              (Efield
+                (Ederef (Etempvar _t (tptr t_struct_list)) t_struct_list) _t
+                (tptr t_struct_list)))
             (Sset _s
-              (Ecast (Ebinop Oadd (Etempvar _s tint) (Etempvar _h tint) tint)
-                tint)))))
+              (Ebinop Oadd (Etempvar _s tint) (Etempvar _h tint) tint)))))
       (Sreturn (Some (Etempvar _s tint))))))
 |}.
 
@@ -71,36 +67,28 @@ Definition f_reverse := {|
                (_v, (tptr t_struct_list)) :: nil);
   fn_body :=
 (Ssequence
-  (Sset _w
-    (Ecast (Ecast (Econst_int (Int.repr 0) tint) (tptr tvoid))
-      (tptr t_struct_list)))
+  (Sset _w (Ecast (Econst_int (Int.repr 0) tint) (tptr tvoid)))
   (Ssequence
-    (Sset _v (Ecast (Etempvar _p (tptr t_struct_list)) (tptr t_struct_list)))
+    (Sset _v (Etempvar _p (tptr t_struct_list)))
     (Ssequence
       (Swhile
         (Etempvar _v (tptr t_struct_list))
         (Ssequence
           (Sset _t
-            (Ecast
-              (Efield
-                (Ederef (Etempvar _v (tptr t_struct_list)) t_struct_list) _t
-                (tptr t_struct_list)) (tptr t_struct_list)))
+            (Efield (Ederef (Etempvar _v (tptr t_struct_list)) t_struct_list)
+              _t (tptr t_struct_list)))
           (Ssequence
             (Sassign
               (Efield
                 (Ederef (Etempvar _v (tptr t_struct_list)) t_struct_list) _t
                 (tptr t_struct_list)) (Etempvar _w (tptr t_struct_list)))
             (Ssequence
-              (Sset _w
-                (Ecast (Etempvar _v (tptr t_struct_list))
-                  (tptr t_struct_list)))
-              (Sset _v
-                (Ecast (Etempvar _t (tptr t_struct_list))
-                  (tptr t_struct_list)))))))
+              (Sset _w (Etempvar _v (tptr t_struct_list)))
+              (Sset _v (Etempvar _t (tptr t_struct_list)))))))
       (Sreturn (Some (Etempvar _w (tptr t_struct_list)))))))
 |}.
 
-(* as produced by Clightgen, version as of 6 jan 2012 ...
+(*
 Definition f_main := {|
   fn_return := tint;
   fn_params := nil;
@@ -115,15 +103,13 @@ Definition f_main := {|
       (Evar _reverse (Tfunction (Tcons (tptr t_struct_list) Tnil)
                        (tptr t_struct_list)))
       ((Evar _three (tarray t_struct_list 3)) :: nil))
-    (Sset _r
-      (Ecast (Etempvar 16%positive (tptr t_struct_list))
-        (tptr t_struct_list))))
+    (Sset _r (Etempvar 16%positive (tptr t_struct_list))))
   (Ssequence
     (Ssequence
       (Scall (Some 17%positive)
         (Evar _sumlist (Tfunction (Tcons (tptr t_struct_list) Tnil) tint))
         ((Etempvar _r (tptr t_struct_list)) :: nil))
-      (Sset _s (Ecast (Etempvar 17%positive tint) tint)))
+      (Sset _s (Etempvar 17%positive tint)))
     (Sreturn (Some (Etempvar _s tint)))))
 |}.
 *)
